refine+crefine: remove valid_arch_mdb_ctes
- replace the ioport_control invariant with archMDBAssertions
- remove lemmas needed only for the invariant
- add corresponding crossing lemmas for caps_of_state based on existing
  older cte_wp_at lemmas

Signed-off-by: Gerwin Klein <gerwin.klein@proofcraft.systems>

proof/refine/ARM/CSpace1_R.thy
@@ -14,6 +14,20 @@ imports
   "AInvs.ArchDetSchedSchedule_AI"
 begin
 
+context Arch begin arch_global_naming
+
+(* No assertion necessary for this architecture. *)
+definition arch_mdb_assert :: "cte_heap \<Rightarrow> bool" where
+  "arch_mdb_assert m \<equiv> True"
+
+end
+
+arch_requalify_consts
+  arch_mdb_assert
+
+defs archMDBAssertions_def:
+  "archMDBAssertions s \<equiv> arch_mdb_assert (ctes_of s)"
+
 context Arch begin global_naming ARM_A (*FIXME: arch-split*)
 
 lemmas final_matters_def = final_matters_def[simplified final_matters_arch_def]
@@ -250,12 +264,28 @@ lemma pspace_relation_cte_wp_at:
 
 lemma pspace_relation_ctes_ofI:
   "\<lbrakk> pspace_relation (kheap s) (ksPSpace s');
-    cte_wp_at ((=) c) slot s; pspace_aligned' s';
+     cte_wp_at ((=) c) slot s; pspace_aligned' s';
      pspace_distinct' s' \<rbrakk>
   \<Longrightarrow> \<exists>cte. ctes_of s' (cte_map slot) = Some cte \<and> cap_relation c (cteCap cte)"
   apply (cases slot, clarsimp)
   apply (drule(3) pspace_relation_cte_wp_at)
   apply (simp add: cte_wp_at_ctes_of)
+  done
+
+lemma pspace_relation_caps_of_state_cross:
+  "\<lbrakk> pspace_relation (kheap s) (ksPSpace s');
+     caps_of_state s slot = Some c; pspace_aligned s; pspace_distinct s \<rbrakk>
+   \<Longrightarrow> \<exists>cte. ctes_of s' (cte_map slot) = Some cte \<and> cap_relation c (cteCap cte)"
+  for s' :: kernel_state
+  by (auto simp: cte_wp_at_caps_of_state
+           intro!: pspace_relation_ctes_ofI pspace_aligned_cross pspace_distinct_cross)
+
+lemma caps_of_state_cross:
+  "\<lbrakk> caps_of_state s slot = Some cap; pspace_aligned s; pspace_distinct s; (s,s') \<in> state_relation \<rbrakk>
+   \<Longrightarrow> \<exists>cap'. cteCaps_of s' (cte_map slot) = Some cap' \<and> cap_relation cap cap'"
+  apply (erule state_relationE)
+  apply (drule (3) pspace_relation_caps_of_state_cross)
+  apply (fastforce simp: cteCaps_of_def)
   done
 
 lemma get_cap_corres_P:
@@ -890,21 +920,13 @@ lemma ctes_of_valid_cap'':
   done
 
 lemma cap_insert_objs' [wp]:
-  "\<lbrace>valid_objs'
-    and valid_cap' cap\<rbrace>
-   cteInsert cap src dest \<lbrace>\<lambda>rv. valid_objs'\<rbrace>"
-  including no_pre
-  apply (simp add: cteInsert_def updateCap_def setUntypedCapAsFull_def bind_assoc split del: if_split)
-  apply (wp setCTE_valid_objs)
-      apply simp
-      apply wp+
-      apply (clarsimp simp: updateCap_def)
-      apply (wp|simp)+
-    apply (rule hoare_drop_imp)+
-    apply wp+
-  apply (rule hoare_strengthen_post[OF getCTE_sp])
+  "\<lbrace>valid_objs' and valid_cap' cap\<rbrace>
+   cteInsert cap src dest
+   \<lbrace>\<lambda>_. valid_objs'\<rbrace>"
+  apply (simp add: cteInsert_def updateCap_def setUntypedCapAsFull_def)
+  apply (wpsimp wp: setCTE_valid_objs | wp getCTE_wp')+
   apply (clarsimp simp: cte_wp_at_ctes_of isCap_simps
-                 dest!: ctes_of_valid_cap'')
+                  dest!: ctes_of_valid_cap'')
   done
 
 lemma cteInsert_weak_cte_wp_at:
@@ -1928,6 +1950,14 @@ lemma pspace_relation_cte_wp_atI:
   apply (erule pspace_relation_cte_wp_atI'[where x=x])
    apply (simp add: cte_wp_at_ctes_of)
   apply assumption
+  done
+
+lemma caps_of_state_rev_cross:
+  "\<lbrakk> ctes_of s' p = Some cte; valid_objs s; (s,s') \<in> state_relation \<rbrakk>
+   \<Longrightarrow> \<exists>cap slot. caps_of_state s slot = Some cap \<and> p = cte_map slot \<and> cap_relation cap (cteCap cte)"
+  apply (erule state_relationE)
+  apply (drule (2) pspace_relation_cte_wp_atI)
+  apply (fastforce simp: cte_wp_at_caps_of_state)
   done
 
 lemma sameRegion_corres:
@@ -5064,6 +5094,15 @@ lemma cte_map_inj_eq':
   done
 
 context begin interpretation Arch . (*FIXME: arch-split*)
+
+(* interface lemma: generic statement, arch-specific proof *)
+lemma archMDBAssertions_cross:
+  "\<lbrakk> valid_arch_mdb (is_original_cap s) (caps_of_state s); valid_arch_state s; valid_objs s;
+     (s, s') \<in> state_relation \<rbrakk>
+   \<Longrightarrow> archMDBAssertions s'"
+  unfolding archMDBAssertions_def
+  by (simp add: arch_mdb_assert_def)
+
 lemma cteInsert_corres:
   notes split_paired_All[simp del] split_paired_Ex[simp del]
         trans_state_update'[symmetric,simp]
@@ -5072,30 +5111,33 @@ lemma cteInsert_corres:
         (valid_objs and pspace_distinct and pspace_aligned and
          valid_mdb and valid_list and K (src\<noteq>dest) and
          cte_wp_at (\<lambda>c. c=Structures_A.NullCap) dest and
-         (\<lambda>s. cte_wp_at (is_derived (cdt s) src c) src s))
+         (\<lambda>s. cte_wp_at (is_derived (cdt s) src c) src s) and valid_arch_state)
         (pspace_distinct' and pspace_aligned' and valid_mdb' and valid_cap' c' and
          cte_wp_at' (\<lambda>c. cteCap c=NullCap) dest')
         (cap_insert c src dest)
         (cteInsert c' src' dest')"
-  (is "corres _ (?P and (\<lambda>s. cte_wp_at _ _ s)) (?P' and cte_wp_at' _ _) _ _")
+  (is "corres _ (?P and (\<lambda>s. cte_wp_at _ _ s) and valid_arch_state) (?P' and cte_wp_at' _ _) _ _")
   using assms
   unfolding cap_insert_def cteInsert_def
   apply simp
+  (* this lemma doesn't use the assertion, but does need to establish it *)
+  apply (rule corres_stateAssert_add_assertion[rotated])
+   apply (rule archMDBAssertions_cross; simp add: valid_mdb_def)
   apply (rule corres_guard_imp)
     apply (rule corres_split[OF get_cap_corres])
       apply (rule corres_split[OF get_cap_corres])
-        apply (rule_tac F="cteCap rv' = NullCap" in corres_gen_asm2)
+        apply (rule_tac F="cteCap oldCTE = NullCap" in corres_gen_asm2)
         apply simp
         apply (rule_tac P="?P and cte_at dest and
                             (\<lambda>s. cte_wp_at (is_derived (cdt s) src c) src s) and
                             cte_wp_at ((=) src_cap) src" and
                         Q="?P' and
-                           cte_wp_at' ((=) rv') (cte_map dest) and
+                           cte_wp_at' ((=) oldCTE) (cte_map dest) and
                            cte_wp_at' ((=) srcCTE) (cte_map src)"
                         in corres_assert_assume)
          prefer 2
          apply (clarsimp simp: cte_wp_at_ctes_of valid_mdb'_def valid_mdb_ctes_def valid_nullcaps_def)
-         apply (case_tac rv')
+         apply (case_tac oldCTE)
          apply (simp add: initMDBNode_def)
          apply (erule allE)+
          apply (erule (1) impE)
@@ -5104,7 +5146,7 @@ lemma cteInsert_corres:
           apply (rule_tac R="\<lambda>r. ?P and cte_at dest and
                             (\<lambda>s. (is_derived (cdt s) src c) src_cap) and
                             cte_wp_at ((=) (masked_as_full src_cap c)) src" and
-                        R'="\<lambda>r. ?P' and cte_wp_at' ((=) rv') (cte_map dest) and
+                        R'="\<lambda>r. ?P' and cte_wp_at' ((=) oldCTE) (cte_map dest) and
                            cte_wp_at' ((=) (CTE (maskedAsFull (cteCap srcCTE) c') (cteMDBNode srcCTE)))
                            (cte_map src)"
                         in corres_split[where r'=dc])
@@ -5168,7 +5210,7 @@ lemma cteInsert_corres:
               apply (thin_tac "machine_state t = s" for s t)+
               apply (case_tac "srcCTE")
               apply (rename_tac src_cap' src_node)
-              apply (case_tac "rv'")
+              apply (case_tac "oldCTE")
               apply (rename_tac dest_node)
               apply (clarsimp simp: in_set_cap_cte_at_swp)
               apply (subgoal_tac "cte_at src a \<and> is_derived (cdt a) src c src_cap")
@@ -5455,7 +5497,7 @@ lemma cteInsert_corres:
               apply clarsimp
               apply (subgoal_tac "mdbRevocable node = revokable' (cteCap srcCTE) c'")
                prefer 2
-               apply (case_tac rv')
+               apply (case_tac oldCTE)
                subgoal by (clarsimp simp add: const_def modify_map_def split: if_split_asm)
               apply simp
               apply (rule revokable_eq, assumption, assumption)
@@ -5468,7 +5510,7 @@ lemma cteInsert_corres:
                                   split:if_splits dest!:cap_master_cap_eqDs)
              apply clarsimp
              apply (case_tac srcCTE)
-             apply (case_tac rv')
+             apply (case_tac oldCTE)
              apply clarsimp
              apply (subgoal_tac "\<exists>cap' node'. ctes_of b (cte_map (aa,bb)) = Some (CTE cap' node')")
               prefer 2
@@ -5494,7 +5536,7 @@ lemma cteInsert_corres:
             apply (wp set_untyped_cap_full_valid_objs set_untyped_cap_as_full_valid_mdb
                set_untyped_cap_as_full_cte_wp_at setUntypedCapAsFull_valid_cap
                setUntypedCapAsFull_cte_wp_at | clarsimp simp: cte_wp_at_caps_of_state| wps)+
-         apply (case_tac rv',clarsimp simp:cte_wp_at_ctes_of maskedAsFull_def)
+         apply (case_tac oldCTE,clarsimp simp:cte_wp_at_ctes_of maskedAsFull_def)
         apply (wp getCTE_wp' get_cap_wp)+
     apply clarsimp
     subgoal by (fastforce elim: cte_wp_at_weakenE)
@@ -5504,7 +5546,7 @@ lemma cteInsert_corres:
   apply (thin_tac "machine_state t = s" for s t)+
   apply (case_tac "srcCTE")
   apply (rename_tac src_cap' src_node)
-  apply (case_tac "rv'")
+  apply (case_tac "oldCTE")
   apply (rename_tac dest_node)
   apply (clarsimp simp: in_set_cap_cte_at_swp)
   apply (subgoal_tac "cte_at src a \<and> is_derived (cdt a) src c src_cap")
